README.md
@@ -5,20 +5,21 @@ Trying Out VeLLVM for a compilers project
     All relevant code is under src/demo
     - exactEqBlocks.v: This is the first part of the demo. It demonstrates basic/syntactic Itree bisimilarity.
     - bisimilarInstructions.v: This is the second part of the demo. It demonstrates bisimilarity of interpreted instructions.
-    - transformPipelineEx.v: This is the final part of the demo. It demonstrates a series of "assembly transformations" and demonstrates the correctness of these transformations by bisimulation on a concrete program.
+    - transformPipelineEx.v: This is the final part of the demo. It demonstrates a series of "assembly transformations" 
+                                and the correctness of these transformations by bisimulation on a concrete program.
 
 ## Build
 coq_makefile -f _CoqProject -o CoqMakefile
 
 make -f CoqMakefile
 
-
-# Directories
+# Notes to self
+## Directories
 /workspaces/VeLLVM-Exploration/
 /home/coq/vellvm/
 /home/coq/InteractionTrees
 
-## How to get VIR from a C program
+### How to get VIR from a C program
 
 #### From C to LLVM
 clang -emit-llvm -S -O0 <filename>.c
